finished Spec.v without the spec_subst operator, instead defining a Pushout type (which we will now try to instantiate by writing an OCaml tactic...)

theories/Spec.v
@@ -172,24 +172,6 @@ Definition model_rest {f T oppred rest}
     | opCons t pf model' => model'
   end.
 
-(* The type of just the ops of spec, with no axiom proofs *)
-Fixpoint spec_ops spec : Type :=
-  match spec with
-    | Spec_Axioms axioms => unit
-    | Spec_Cons f T oppred rest =>
-      OpCons T oppred (fun t pf => spec_ops (rest t pf))
-  end.
-
-(* Extract just the ops from a model of a spec *)
-Fixpoint extract_spec_ops {spec} : spec_model spec -> spec_ops spec :=
-  match spec return spec_model spec -> spec_ops spec with
-    | Spec_Axioms axioms => fun _ => tt
-    | Spec_Cons f T oppred rest =>
-      fun model =>
-        let (t,pf,model') := model in
-        opCons t pf (extract_spec_ops model')
-  end.
-
 
 (*** Spec Examples ***)
 
@@ -324,100 +306,45 @@ Definition spec_example_model_natmonoid
 
 (*** Interpretations ***)
 
-(* An interpretation from spec1 into spec2 is a function from models of spec2 to
-models of spec1 where the returned ops for spec2 do not depend on the proofs of
-the axioms of spec1; this condition is formalized by saying that there is a
-function from the ops of spec2 to those of spec1 that is related to the model
-function by extract_spec_ops. *)
-Inductive Interpretation spec1 spec2 :=
-| mkInterp (model_f: spec_model spec2 -> spec_model spec1)
-           (ops_f: spec_ops spec2 -> spec_ops spec1)
-           (interp_pf: forall model2,
-                         extract_spec_ops (model_f model2) =
-                         ops_f (extract_spec_ops model2))
-.
-
-Arguments mkInterp {spec1 spec2} model_f ops_f interp_pf.
-
-(* Apply the model function of an interpretation *)
-Definition map_model {spec1 spec2} (i: Interpretation spec1 spec2) :
-           spec_model spec2 -> spec_model spec1 :=
-  let (model_f,_,_) := i in model_f.
-
-(* Apply the ops function of an interpretation *)
-Definition map_ops {spec1 spec2} (i: Interpretation spec1 spec2) :
-           spec_ops spec2 -> spec_ops spec1 :=
-  let (_,ops_f,_) := i in ops_f.
-
-(* Extract the interp_pf from an interpretation *)
-Definition get_interp_pf {spec1 spec2} (i: Interpretation spec1 spec2) :
-  forall model2, extract_spec_ops (map_model i model2) =
-                 map_ops i (extract_spec_ops model2) :=
-  match i return forall model2, extract_spec_ops (map_model i model2) =
-                                map_ops i (extract_spec_ops model2) with
-
-    | mkInterp _ _ interp_pf => interp_pf
-  end.
+(* An interpretation from spec1 into spec2 is just a function from models of
+spec2 to models of spec1. *)
+Definition Interpretation spec1 spec2 :=
+  spec_model spec2 -> spec_model spec1.
 
 (* The identity interpretation *)
-Program Definition interp_id (spec:Spec) : Interpretation spec spec :=
-  mkInterp id _ _.
+Program Definition interp_id (spec:Spec) : Interpretation spec spec := id.
 
 (* Composing interpretations *)
 Program Definition interp_compose {s1 s2 s3}
            (i2: Interpretation s2 s3) (i1: Interpretation s1 s2) :
-  Interpretation s1 s3 :=
-  mkInterp (fun model3 => map_model i1 (map_model i2 model3))
-           (fun ops3 => map_ops i1 (map_ops i2 ops3))
-           _
-.
-Obligation 1.
-destruct i1; destruct i2. unfold map_model, map_ops.
-rewrite interp_pf. rewrite interp_pf0. reflexivity.
-Qed.
+  Interpretation s1 s3 := fun model3 => i1 (i2 model3).
 
 (* Build an interpretation between the tails of two specs that have the same
 head into an interpretation between the whole of the two specs *)
-Program Definition interp_cons f T (oppred: OpPred T)
-           {spec1 spec2 : forall t, oppred t -> Spec}
-           (i: forall t pfs, Interpretation (spec1 t pfs) (spec2 t pfs)) :
+Definition interp_cons f T (oppred: OpPred T)
+        {spec1 spec2 : forall t, oppred t -> Spec}
+        (i: forall t pfs, Interpretation (spec1 t pfs) (spec2 t pfs)) :
   Interpretation (Spec_Cons f T oppred spec1)
                  (Spec_Cons f T oppred spec2) :=
-  mkInterp (fun model2:spec_model (Spec_Cons f T oppred spec2) =>
-              let (t,pf,rest) := model2 in
-              opCons t pf (map_model (i _ _) rest))
-           (fun ops2:spec_ops (Spec_Cons f T oppred spec2) =>
-              let (t,pf,rest) := ops2 in
-              opCons t pf (map_ops (i _ _) rest))
-           _.
-Obligation 1.
-destruct model2. destruct (i t pf). unfold map_model, map_ops.
-rewrite interp_pf. reflexivity.
-Qed.
+  fun model2:spec_model (Spec_Cons f T oppred spec2) =>
+    let (t,pf,rest) := model2 in
+    opCons t pf (i _ _ rest).
 
 (* Take an interpretation from spec1 to spec2 and cons an op onto spec2 *)
-Program Definition interp_cons_r f T (oppred: OpPred T)
+Definition interp_cons_r f T (oppred: OpPred T)
            {spec1} {spec2: forall t, oppred t -> Spec}
            (i: forall t pfs, Interpretation spec1 (spec2 t pfs)) :
   Interpretation spec1 (Spec_Cons f T oppred spec2) :=
-  mkInterp (fun model2:spec_model (Spec_Cons f T oppred spec2) =>
-              let (t,pf,rest) := model2 in
-              map_model (i t pf) rest)
-           (fun ops2:spec_ops (Spec_Cons f T oppred spec2) =>
-              let (t,pf,rest) := ops2 in
-              map_ops (i t pf) rest)
-           _.
-Obligation 1.
-destruct model2. destruct (i t pf). unfold map_model, map_ops.
-rewrite interp_pf. reflexivity.
-Qed.
+  fun model2:spec_model (Spec_Cons f T oppred spec2) =>
+    let (t,pf,rest) := model2 in
+    i t pf rest.
 
 
 (*** Example Interpretations ***)
 
 (* Interpret T as nat and n as n for spec_example_3 into spec_example_2 *)
 Program Definition interp_example_3_2__models :
-  spec_model spec_example_2 -> spec_model spec_example_3 :=
+  Interpretation spec_example_3 spec_example_2 :=
   (fun (model2:spec_model spec_example_2) =>
      match model2 with
        | opCons n n__proof ax_proofs =>
@@ -427,190 +354,24 @@ Program Definition interp_example_3_2__models :
                     _)) : spec_model spec_example_3
      end).
 
-Program Definition interp_example_3_2 : Interpretation spec_example_3 spec_example_2 :=
-  mkInterp
-    interp_example_3_2__models
-    (fun (ops2:spec_ops spec_example_2) =>
-       match ops2 with
-         | opCons n n__proof tt =>
-           (opCons
-              (oppred:=Pred_Eq nat) _ _
-              (opCons (oppred:=Pred_Trivial) _ _ tt))
-       end)
-    (*
-    (fun ops2 =>
-       match ops2 with
-         | opCons n n__proof ax_proofs =>
-           (opCons
-              (oppred:=Pred_Eq nat) nat eq_refl
-              (opCons (oppred:=Pred_Trivial) n _
-                      _))
-       end)
-     *)
-    (fun (model:spec_model spec_example_2) =>
-    $(repeat (let t := fresh t in
-              let pf := fresh pf in
-              destruct model as [t pf model]);
-     reflexivity)$)
-.
+
+(*** Pushouts ***)
+
+(* A pushout of i1:spec->spec1 and i2:spec->spec2 is some spec' and two
+interpretations i1':spec1->spec' and i2':spec2->spec' such that compose i1 i1'
+equals compose i2 i2'. (Technically, a pushout is the "least" such spec, but it
+is not really practical nor necessary to prove the leastness inside Coq) *)
+Record Pushout {spec spec1 spec2} (i1: Interpretation spec spec1)
+          (i2: Interpretation spec spec2) : Type :=
+  {spec': Spec;
+   i1': Interpretation spec1 spec';
+   i2': Interpretation spec2 spec';
+   pushout_pf: forall model', i1 (i1' model') = i2 (i2' model') }.
 
 
-(*** Appending Specs ***)
+(*** Spec Extensions ***)
 
-(* Prepend axioms to the axioms already in a spec *)
-Fixpoint spec_prepend_axioms axioms1 spec : Spec :=
-  match spec with
-    | Spec_Axioms axioms2 => Spec_Axioms (axioms1 ++ axioms2)
-    | Spec_Cons f T oppred rest =>
-      Spec_Cons f T oppred (fun t pf => spec_prepend_axioms axioms1 (rest t pf))
-  end.
-
-Lemma conjoin_axioms_prepend1 axioms1 axioms2 :
-  conjoin_axioms (axioms1 ++ axioms2) -> conjoin_axioms axioms1.
-  induction axioms1.
-  intros; constructor.
-  intros; destruct a; destruct (conjoin_axioms_destruct _ _ _ H).
-  apply conjoin_axioms_cons; [ assumption | apply IHaxioms1; assumption ].
-Qed.
-
-Lemma conjoin_axioms_prepend2 axioms1 axioms2 :
-  conjoin_axioms (axioms1 ++ axioms2) -> conjoin_axioms axioms2.
-  induction axioms1; intros.
-  assumption.
-  apply IHaxioms1.
-  destruct a; destruct (conjoin_axioms_destruct _ _ _ H); assumption.
-Qed.
-
-Lemma conjoin_axioms_prepend_inv axioms1 axioms2 :
-  conjoin_axioms axioms1 -> conjoin_axioms axioms2 ->
-  conjoin_axioms (axioms1 ++ axioms2).
-  induction axioms1; intros.
-  assumption.
-  destruct a; destruct (conjoin_axioms_destruct _ _ _ H).
-  apply conjoin_axioms_cons; [ | apply IHaxioms1 ]; assumption.
-Qed.
-
-(* The interpretation from axioms to the result of prepending them to a spec *)
-Fixpoint prepend_axioms_interp1 axioms1 spec :
-  Interpretation (Spec_Axioms axioms1) (spec_prepend_axioms axioms1 spec) :=
-  match spec return Interpretation (Spec_Axioms axioms1) (spec_prepend_axioms axioms1 spec) with
-    | Spec_Axioms axioms2 =>
-      mkInterp
-        (fun (model12 : spec_model (spec_prepend_axioms _ (Spec_Axioms _))) =>
-           conjoin_axioms_prepend1 axioms1 axioms2 model12
-           : spec_model (Spec_Axioms _))
-        id (fun _ => eq_refl)
-    | Spec_Cons f T oppred rest =>
-      interp_cons_r f T oppred
-                    (fun t pf => prepend_axioms_interp1 axioms1 (rest t pf))
-  end.
-
-(* The interpretation from any spec to the result of prepending axioms to it *)
-Fixpoint prepend_axioms_interp2 axioms1 spec :
-  Interpretation spec (spec_prepend_axioms axioms1 spec) :=
-  match spec return Interpretation spec (spec_prepend_axioms axioms1 spec) with
-    | Spec_Axioms axioms2 =>
-      mkInterp (conjoin_axioms_prepend2 axioms1 axioms2
-                : spec_model (Spec_Axioms _) -> spec_model (Spec_Axioms _))
-               id (fun _ => eq_refl)
-    | Spec_Cons f T oppred rest =>
-      interp_cons f T oppred (fun t pf => prepend_axioms_interp2 axioms1 (rest t pf))
-  end.
-
-(* Append one spec after another, where the spec being appended can depend on
-the ops of the spec it is coming after *)
-Fixpoint spec_append spec1 : (spec_ops spec1 -> Spec) -> Spec :=
-  match spec1 return (spec_ops spec1 -> Spec) -> Spec with
-    | Spec_Axioms axioms1 =>
-      fun spec2 => spec_prepend_axioms axioms1 (spec2 tt)
-    | Spec_Cons f T oppred rest =>
-      fun spec2 =>
-        Spec_Cons f T oppred
-                    (fun t pf =>
-                       spec_append (rest t pf)
-                                   (fun ops1 =>
-                                      spec2 (opCons t pf ops1)))
-  end.
-
-(* The interpretation from a spec to the result of prepending another spec to it *)
-Fixpoint interp_append1 spec1 :
-  forall spec2, Interpretation spec1 (spec_append spec1 spec2) :=
-  match spec1 return
-        forall spec2, Interpretation spec1 (spec_append spec1 spec2) with
-    | Spec_Axioms axioms1 =>
-      fun spec2 => prepend_axioms_interp1 axioms1 (spec2 tt)
-    | Spec_Cons f T oppred rest =>
-      fun spec2 =>
-        interp_cons f T oppred
-                    (fun t pf =>
-                       interp_append1 (rest t pf)
-                                      (fun ops1 => spec2 (opCons t pf ops1)))
-  end.
-
-(* Extract a model for spec2 from a model for (spec_append spec1 spec2). This
-function is essentially a dependent interpretation, i.e., an interpretation from
-spec2 to (spec_append spec1 spec2) but where the contents of spec2 can depend on
-the spec1 ops contained in the model for (spec_append spec1 spec2) that is
-passed to the interpretation. *)
-Fixpoint interp_append2_model spec1 :
-  forall spec2 (model12: spec_model (spec_append spec1 spec2)),
-    spec_model (spec2 (map_ops (interp_append1 spec1 spec2) (extract_spec_ops model12))) :=
-  match spec1 with
-    | Spec_Axioms axioms1 =>
-      fun spec2 model12 =>
-        match (map_ops (interp_append1 (Spec_Axioms _) spec2)
-                       (extract_spec_ops model12)) as ops1
-              return spec_model (spec2 ops1) with
-          | tt => map_model (prepend_axioms_interp2 _ _) model12
-        end
-    | Spec_Cons f T oppred rest =>
-      fun spec2 model12 =>
-        match model12
-              return spec_model
-                       (spec2
-                          (map_ops (interp_append1 _ spec2)
-                                   (@extract_spec_ops
-                                      (Spec_Cons f T oppred _)
-                                      model12))) with
-          | opCons t pf model12' =>
-            interp_append2_model (rest t pf)
-                                (fun ops1 => spec2 (opCons t pf ops1)) model12'
-        end
-  end.
-
-(* The ops portion of interp_append2_model *)
-Fixpoint interp_append2_ops spec1 :
-  forall spec2 (ops12: spec_ops (spec_append spec1 spec2)),
-    spec_ops (spec2 (map_ops (interp_append1 spec1 spec2) ops12)) :=
-  match spec1 with
-    | Spec_Axioms axioms1 =>
-      fun spec2 ops12 =>
-        match map_ops (interp_append1 (Spec_Axioms _) spec2) ops12 as ops1
-              return spec_ops (spec2 ops1) with
-          | tt => map_ops (prepend_axioms_interp2 _ _) ops12
-        end
-    | Spec_Cons f T oppred rest =>
-      fun spec2 ops12 =>
-        match ops12
-              return spec_ops
-                       (spec2 (map_ops (interp_append1 _ spec2) ops12)) with
-          | opCons t pf ops12' =>
-            interp_append2_ops (rest t pf)
-                                (fun ops1 => spec2 (opCons t pf ops1)) ops12'
-        end
-  end.
-
-(* The proof associated with interp_append2_model/ops *)
-Lemma interp_append2_interp_pf spec1 spec2 model12 :
-  extract_spec_ops (interp_append2_model spec1 spec2 model12) =
-  interp_append2_ops spec1 spec2 (extract_spec_ops model12).
-  revert spec2 model12; induction spec1; intros.
-  unfold interp_append2_model, interp_append2_ops.
-  destruct (map_ops (interp_append1 (Spec_Axioms axioms) spec2)
-                    (extract_spec_ops model12)).
-  apply (get_interp_pf _).
-  admit. (* FIXME HERE NOW *)
-Qed.
+(* FIXME HERE: formalize SpecExtension (i.e., sub-specs) *)
 
 
 (*** Spec Overlap ***)
@@ -788,530 +549,15 @@ Ltac prove_spec_overlapN n :=
   end.
 
 
-(*** Spec Substitution ***)
-
-(* Helper for spec_subtract: return all axioms in the axioms1 list that do not
-overlap with the axioms in axioms2 *)
-Fixpoint axioms_subtract axioms1 axioms2
-         (overlap: AxiomOverlap axioms1 axioms2) : list SpecAxiom :=
-  match overlap with
-    | AxiomOverlap_base => []
-    | AxiomOverlap_eq ax_name ax_tp axioms1 axioms2 overlap' =>
-      axioms_subtract axioms1 axioms2 overlap'
-    | AxiomOverlap_neq1 ax_name ax_tp axioms1' axioms2' not_in overlap' =>
-      (specAxiom ax_name ax_tp)
-        :: axioms_subtract axioms1' axioms2' overlap'
-    | AxiomOverlap_neq2 ax_name ax_tp axioms1' axioms2' not_in overlap' =>
-      axioms_subtract axioms1' axioms2' overlap'
-  end.
-
-(* If you subtract axioms2 from axioms1 and then add them back again you can
-prove the original axioms1. *)
-Lemma axioms_subtract_interp axioms1 axioms2 overlap :
-  conjoin_axioms axioms2 ->
-  conjoin_axioms (axioms_subtract axioms1 axioms2 overlap) ->
-  conjoin_axioms axioms1.
-  induction overlap; intros.
-  trivial.
-  destruct (conjoin_axioms_destruct _ _ _ H).
-  apply conjoin_axioms_cons; [ assumption | apply IHoverlap; assumption ].
-  destruct (conjoin_axioms_destruct _ _ _ H0).
-  apply conjoin_axioms_cons; [ assumption | apply IHoverlap; assumption ].
-  destruct (conjoin_axioms_destruct _ _ _ H).
-  apply IHoverlap; assumption.
-Qed.
-
-(* Subtract the overlapping ops and axioms in spec2 from spec1. Note that this
-operation requires ops for spec2. *)
-Fixpoint spec_subtract spec1 spec2 (overlap: SpecOverlap spec1 spec2) :
-  spec_ops spec2 -> Spec :=
-  match overlap in SpecOverlap spec1 spec2 return spec_ops spec2 -> Spec with
-    | SpecOverlap_base axioms1 axioms2 overlap' =>
-      fun _ => Spec_Axioms (axioms_subtract axioms1 axioms2 overlap')
-    | SpecOverlap_eq f T oppred rest1 rest2 overlap' =>
-      fun ops2 =>
-        let (t,pf,ops2') := ops2 in
-        spec_subtract (rest1 t pf) (rest2 t pf) (overlap' t pf) ops2'
-    | SpecOverlap_neq1 f1 T1 oppred1 rest1 spec2 not_in overlap' =>
-      fun ops2 =>
-        Spec_Cons f1 T1 oppred1
-                    (fun t pf =>
-                       spec_subtract (rest1 t pf) spec2 (overlap' t pf) ops2)
-    | SpecOverlap_neq2 f2 T2 oppred2 rest2 spec1 not_in overlap' =>
-      fun ops2 =>
-        let (t,pf,ops2') := ops2 in
-        spec_subtract spec1 (rest2 t pf) (overlap' t pf) ops2'
-  end.
-
-(* If you subtract spec2 from spec1 then you can recover a model of spec1 if you
-have models for spec2 and for the subtraction. This is like a binary
-interpretation from spec1 to the pair (spec2, spec1-spec2). *)
-Fixpoint interp_spec_subtract_model spec1 spec2 overlap :
-  forall (model2:spec_model spec2),
-  spec_model (spec_subtract spec1 spec2 overlap (extract_spec_ops model2)) ->
-  spec_model spec1 :=
-  match overlap in SpecOverlap spec1 spec2
-        return forall model2,
-                 spec_model (spec_subtract spec1 spec2 overlap
-                                           (extract_spec_ops model2)) ->
-                 spec_model spec1 with
-    | SpecOverlap_base axioms1 axioms2 overlap' =>
-      fun model2 model21 =>
-        axioms_subtract_interp axioms1 axioms2 overlap' model2 model21
-    | SpecOverlap_eq f T oppred rest1 rest2 overlap' =>
-      fun model2 =>
-        match model2 return
-              spec_model (spec_subtract
-                          _ _ (SpecOverlap_eq _ _ _ _ _ overlap')
-                          (@extract_spec_ops
-                             (Spec_Cons f T oppred rest2)
-                             model2)) ->
-              spec_model (Spec_Cons f T oppred rest1) with
-          | opCons t pf model2' =>
-            fun model21 =>
-              opCons t pf (interp_spec_subtract_model _ _ (overlap' t pf)
-                                                      model2' model21)
-        end
-    | SpecOverlap_neq1 f1 T1 oppred1 rest1 spec2 not_in overlap' =>
-      fun model2 model21 =>
-        match model21 return spec_model (Spec_Cons f1 T1 oppred1 rest1) with
-          | opCons t pf model21' =>
-            opCons t pf (interp_spec_subtract_model _ _ (overlap' t pf)
-                                                    model2 model21')
-        end
-    | SpecOverlap_neq2 f2 T2 oppred2 rest2 spec1 not_in overlap' =>
-      fun model2 =>
-        match model2 return
-              spec_model (spec_subtract
-                          _ _ (SpecOverlap_neq2 _ _ _ _ _ _ overlap')
-                          (@extract_spec_ops
-                             (Spec_Cons f2 T2 oppred2 rest2)
-                             model2)) ->
-              spec_model spec1 with
-          | opCons t pf model2' =>
-            fun model21 =>
-              interp_spec_subtract_model _ _ (overlap' t pf) model2' model21
-        end
-  end.
-
-(* Same as interp_spec_subtract_model but for ops *)
-Fixpoint interp_spec_subtract_ops spec1 spec2 overlap :
-  forall (ops2:spec_ops spec2),
-  spec_ops (spec_subtract spec1 spec2 overlap ops2) ->
-  spec_ops spec1 :=
-  match overlap in SpecOverlap spec1 spec2
-        return forall ops2,
-                 spec_ops (spec_subtract spec1 spec2 overlap ops2) ->
-                 spec_ops spec1 with
-    | SpecOverlap_base axioms1 axioms2 overlap' =>
-      fun ops2 ops21 => tt
-    | SpecOverlap_eq f T oppred rest1 rest2 overlap' =>
-      fun ops2 =>
-        match ops2 return
-              spec_ops (spec_subtract
-                          _ _ (SpecOverlap_eq _ _ _ _ _ overlap') ops2) ->
-              spec_ops (Spec_Cons f T oppred rest1) with
-          | opCons t pf ops2' =>
-            fun ops21 =>
-              opCons t pf (interp_spec_subtract_ops _ _ (overlap' t pf)
-                                                    ops2' ops21)
-        end
-    | SpecOverlap_neq1 f1 T1 oppred1 rest1 spec2 not_in overlap' =>
-      fun ops2 ops21 =>
-        match ops21 return spec_ops (Spec_Cons f1 T1 oppred1 rest1) with
-          | opCons t pf ops21' =>
-            opCons t pf (interp_spec_subtract_ops _ _ (overlap' t pf)
-                                                  ops2 ops21')
-        end
-    | SpecOverlap_neq2 f2 T2 oppred2 rest2 spec1 not_in overlap' =>
-      fun ops2 =>
-        match ops2 return
-              spec_ops (spec_subtract
-                          _ _ (SpecOverlap_neq2 _ _ _ _ _ _ overlap') ops2) ->
-              spec_ops spec1 with
-          | opCons t pf ops2' =>
-            fun ops21 =>
-              interp_spec_subtract_ops _ _ (overlap' t pf) ops2' ops21
-        end
-  end.
-
-Lemma interp_spec_subtract_proof spec1 spec2 overlap :
-  forall model2 model21,
-    extract_spec_ops
-      (interp_spec_subtract_model spec1 spec2 overlap model2 model21)
-    = interp_spec_subtract_ops spec1 spec2 overlap (extract_spec_ops model2)
-                               (extract_spec_ops model21).
-  induction overlap; intros; admit.
-Qed.
+(* FIXME HERE: define spec_of_overlap, which uses a SpecOverlap spec1 spec2 to
+construct a spec that is an extension of both spec1 and spec2 *)
 
 
-(* Build a spec using spec substitution *)
-Definition spec_subst {spec spec1 spec2}
-           (overlap: SpecOverlap spec spec1) (i: Interpretation spec1 spec2) : Spec :=
-  spec_append spec2
-              (fun ops2 =>
-                 spec_subtract spec spec1 overlap (map_ops i ops2)).
+(*** Proving Isomorphisms between Type Classes and Specs ***)
 
-(* FIXME HERE NOW: looks like doing the proof for interp_spec_subst1 is going to
-require UIP, since the second argument of interp_spec_subtract_model is
-dependent on the first, which needs to be cast using the interp_pf of i.
-
-IDEA: maybe this could work via induction on spec2 followed by induction on
-spec1, so that the interp_pf is used to cast each op separately instead of for
-the whole spec substitution. The latter induction, on spec1, would be a version
-of interp_spec_subtract_model that also takes i as an argument. *)
-
-Definition interp_spec_subst1_model spec spec1 spec2 overlap i :
-  spec_model (@spec_subst spec spec1 spec2 overlap i) ->
-  spec_model spec.
-  revert spec spec1 overlap i; induction spec2; unfold spec_subst; intros.
-  apply (interp_spec_subtract_model
-           _ _ overlap (map_model i (map_model (interp_append1 _ _) X))).
-  rewrite (get_interp_pf i).
-  rewrite (get_interp_pf (interp_append1 _ _)).
-  apply (interp_append2_model _ _ X).
-  destruct X0 as [t pf model'].
-  refine (X t pf _ _ overlap
-            (mkInterp (fun model =>
-                         map_model i (opCons (U:=fun t pf => spec_model (rest t pf)) t pf model))
-                      (fun ops =>
-                         map_ops i (opCons (U:=fun t pf => spec_ops (rest t pf)) t pf ops)) _)
-            model').
-  intro; apply (get_interp_pf i).
-Defined.
-
-Print interp_spec_subst1_model.
-
-Definition interp_spec_subst1_ops spec spec1 spec2 overlap i :
-  spec_ops (@spec_subst spec spec1 spec2 overlap i) ->
-  spec_ops spec.
-  revert spec spec1 overlap i; induction spec2; unfold spec_subst; intros.
-  apply (interp_spec_subtract_ops
-           _ _ overlap (map_ops i (map_ops (interp_append1 _ _) X))).
-  apply (interp_append2_ops _ _ X).
-  destruct X0 as [t pf ops'].
-  refine (X t pf _ _ overlap
-            (mkInterp (fun model =>
-                         map_model i (opCons (U:=fun t pf => spec_model (rest t pf)) t pf model))
-                      (fun ops =>
-                         map_ops i (opCons (U:=fun t pf => spec_ops (rest t pf)) t pf ops)) _)
-            ops').
-  intro; apply (get_interp_pf i).
-Defined.
-
-
-
-Program Definition interp_spec_subst1 spec spec1 spec2 overlap i :
-  Interpretation spec (@spec_subst spec spec1 spec2 overlap i) :=
-  mkInterp (interp_spec_subst1_model spec spec1 spec2 overlap i)
-           (interp_spec_subst1_ops spec spec1 spec2 overlap i)
-           _.
-Obligation 1.
-revert spec spec1 overlap i model2; induction spec2; intros.
-*)
-
-
-(* Build the interpretation from spec1 to the result of applying spec
-substitution to spec1 *)
-Program Definition spec_subst_interp1 {spec spec1 spec2} overlap i :
-  Interpretation spec (@spec_subst spec spec1 spec2 overlap i) :=
-  mkInterp
-    (fun model =>
-       interp_spec_subtract_model
-         _ _ overlap
-         (map_model i (map_model (interp_append1 _ _) model))
-         (interp_append2_model _ _ model))
-    (fun ops =>
-       interp_spec_subtract_ops
-         _ _ overlap
-         (map_ops i (map_ops (interp_append1 _ _) ops))
-         (interp_append2_ops _ _ ops))
-    _.
-Preterm.
-Obligation 1.
-f_equal.
-rewrite (get_interp_pf i).
-rewrite (get_interp_pf (interp_append1 spec2 _)).
-reflexivity.
-Defined.
-Obligation 2.
-rewrite interp_spec_subtract_proof.
-
-induction spec2.
-
-f_equal.
-rewrite (get_interp_pf i (map_model (interp_append1 spec2 _ ) model2)).
-
-re
-
-fold (spec_subtract spec spec1 overlap).
-
-  unfold spec_subst.
-  eapply interp_append; intros.
-  apply spec_subtract_interp_model.
-  apply (map_model i _ H).
-  apply H0.
-Defined.
-
-(* Build the interpretation from spec2 to the result of applying any spec
-substitution using an interpretation into spec2 *)
-Definition spec_subst_interp2 {spec spec1 spec2} overlap i :
-  Interpretation spec2 (@spec_subst spec spec1 spec2 overlap i) :=
-  interp_append1 _ _.
-
-
-(*** Quantifying over the Ops of a Spec ***)
-
-Definition ForallOp T (oppred: OpPred T) : (forall t, oppred t -> Type) -> Type :=
-  match oppred return (forall t, sats_op_pred oppred t -> Type) -> Type with
-    | Pred_Trivial => fun A => forall t, A t I
-    | _ => fun A => forall t pf, A t pf
-  end.
-
-Definition LambdaOp T oppred : forall body_tp, (forall t pf, body_tp t pf) ->
-                                               ForallOp T oppred body_tp :=
-  match oppred return forall body_tp, (forall t pf, body_tp t pf) ->
-                                      ForallOp T oppred body_tp with
-    | Pred_Trivial => fun body_tp body => fun t => body t I
-    | _ => fun body_tp body => fun t pf => body t pf
-  end.
-
-Definition replace_op_proof T (oppred: OpPred T) : forall t, oppred t -> oppred t :=
-  match oppred return forall t, sats_op_pred oppred t ->
-                                sats_op_pred oppred t with
-    | Pred_Trivial => fun t _ => I
-    | _ => fun t pf => pf
-  end.
-
-(* Helper: all proofs of True are equal *)
-Definition True_eq (pf1: True) : forall pf2, pf1 = pf2 :=
-  match pf1 return forall pf2, pf1 = pf2 with
-    | I => fun pf2 => match pf2 return I = pf2 with I => eq_refl end end.
-
-(* Helper: all elements of unit are equal *)
-Definition unit_eq (u1: unit) : forall u2, u1 = u2 :=
-  match u1 return forall u2, u1 = u2 with
-    | tt => fun u2 => match u2 return tt = u2 with tt => eq_refl end end.
- 
-(* Replacing an op proof yields an equal proof (because a proof of True is a
-proof of True) *)
-Definition replace_op_proof_eq T (oppred: OpPred T) :
-  forall t pf, pf = replace_op_proof T oppred t pf :=
-  match oppred return forall t pf, pf = replace_op_proof T oppred t pf with
-    | Pred_Trivial => fun t _ => True_eq _ _
-    | _ => fun t pf => eq_refl
-  end.
-
-(* Apply an op function to an op and its proof *)
-Definition ApplyOp T (oppred: OpPred T) :
-  forall body_tp, ForallOp T oppred body_tp ->
-                  forall t pf, body_tp t (replace_op_proof T oppred t pf) :=
-  match oppred return forall body_tp,
-                        ForallOp T oppred body_tp ->
-                        forall t pf, body_tp t (replace_op_proof T oppred t pf) with
-    | Pred_Trivial => fun body_tp body t pf => body t
-    | _ => fun body_tp body t pf => body t pf
-  end.
-
-(* The type of Curried functions on the ops of spec *)
-Fixpoint ForallOps spec : (spec_ops spec -> Type) -> Type :=
-  match spec with
-    | Spec_Axioms _ => fun body_tp => body_tp tt
-    | Spec_Cons f T oppred rest =>
-      fun body_tp =>
-        ForallOp T oppred
-                 (fun t pf => ForallOps (rest t pf)
-                                        (fun ops => body_tp (ops_cons t pf ops)))
-  end.
-
-(* The type of Curried predicates on the ops of spec *)
-Definition OpsPred spec : Type := ForallOps spec (fun _ => Prop).
-
-(* Build a ForallOps function *)
-Fixpoint LambdaOps spec : forall body_tp, (forall ops, body_tp ops) ->
-                                          ForallOps spec body_tp :=
-  match spec return forall body_tp, (forall ops, body_tp ops) ->
-                                    ForallOps spec body_tp with
-    | Spec_Axioms _ =>
-      fun body_tp body => body tt
-    | Spec_Cons f T oppred rest =>
-      fun body_tp body =>
-        LambdaOp T oppred _
-                 (fun t pf =>
-                    LambdaOps (rest t pf) _ (fun ops => body (ops_cons t pf ops)))
-  end.
-
-(* Replace all the trivial True proofs in a spec_ops with I *)
-Fixpoint replace_op_proofs spec : spec_ops spec -> spec_ops spec :=
-  match spec with
-    | Spec_Axioms _ => fun ops => ops
-    | Spec_Cons f T oppred rest =>
-      fun ops =>
-        ops_cons (ops_head ops)
-                 (replace_op_proof T oppred _ (ops_proof ops))
-                 (replace_op_proofs (rest _ _)
-                                    (rew [fun pf => spec_ops (rest _ pf)]
-                                         replace_op_proof_eq T oppred _ _
-                                         in (ops_rest ops)))
-  end.
-
-(* Replacing all the trivial proofs yields an equal ops list *)
-Lemma replace_op_proofs_eq spec ops : replace_op_proofs spec ops = ops.
-  induction spec.
-  reflexivity.
-  unfold replace_op_proofs; fold replace_op_proofs.
-  destruct ops as [t ops]; destruct ops as [pf ops].
-  unfold ops_head; unfold ops_proof; unfold ops_rest; unfold ops_cons;
-    unfold projT1; unfold projT2.
-  destruct oppred; unfold replace_op_proof; unfold replace_op_proof_eq;
-    rewrite H; unfold eq_rect;
-    [ destruct pf | | ]; reflexivity.
-Qed.
-
-(* Apply a Curried predicate to some candidate ops for spec *)
-Fixpoint ApplyOps spec : forall A, (ForallOps spec A) ->
-                                   forall ops, A (replace_op_proofs spec ops) :=
-  match spec return forall A, (ForallOps spec A) ->
-                              forall ops, A (replace_op_proofs spec ops) with
-    | Spec_Axioms _ =>
-      fun A body ops => rew [A] (unit_eq _ _) in body
-    | Spec_Cons f T oppred rest =>
-      fun A body ops =>
-        ApplyOps
-          (rest (ops_head ops)
-                (replace_op_proof T oppred _ (ops_proof ops)))
-          (fun ops => A (ops_cons _ _ ops))
-          (ApplyOp T oppred _ body (ops_head ops) (ops_proof ops))
-          (rew [fun pf => spec_ops (rest _ pf)]
-               replace_op_proof_eq T oppred _ _ in ops_rest ops)
-  end.
-
-
-(*** Types / Typeclasses Represented by Specs ***)
-
-(* FIXME: remove IsoToSpec and IsoInterpretation, and possibly ForallOps *)
-
-(* Whether P is isomorphic to spec *)
-Class IsoToSpec spec (P: OpsPred spec) : Prop :=
-  spec_iso: forall ops, ApplyOps spec _ P ops <-> spec_model spec ops.
-
-(* An IsoInterpretation is an interpretation between type classes / type
-functions that are isomorphic to specs *)
-Definition IsoInterpretation {spec1 P1} (iso1: IsoToSpec spec1 P1)
-           {spec2 P2} (iso2: IsoToSpec spec2 P2)
-           (ops_f: spec_ops spec2 -> spec_ops spec1) : Type :=
-  ForallOps spec2 (fun ops2 => ApplyOps spec2 _ P2 ops2 ->
-                               ApplyOps spec1 _ P1 (ops_f ops2)).
-
-(* Turn an interpretation from spec1 to spec2 into a function from a predicate
-isomorphic to spec2 to a predicate ismorphic to spec1 *)
-Definition toIsoInterp {spec1 P1} {iso1: IsoToSpec spec1 P1}
-           {spec2 P2} {iso2: IsoToSpec spec2 P2}
-           (i: Interpretation spec1 spec2) :
-  IsoInterpretation iso1 iso2 (map_ops i) :=
-  LambdaOps spec2 _ (fun ops2 p2 =>
-                       proj2 (spec_iso (map_ops i ops2))
-                             (map_model i ops2 (proj1 (spec_iso ops2) p2))).
-
-(* Turn an IsoInterpretation into an Interpretation *)
-Definition fromIsoInterp {spec1 P1} {iso1: IsoToSpec spec1 P1}
-           {spec2 P2} {iso2: IsoToSpec spec2 P2} {ops_f}
-           (i: IsoInterpretation iso1 iso2 ops_f) :
-  Interpretation spec1 spec2 :=
-  mkInterp ops_f (fun ops2 model2 =>
-                    proj1 (spec_iso (ops_f ops2))
-                          (rew [fun ops => ApplyOps spec1 _ P1 (ops_f ops)]
-                               (replace_op_proofs_eq _ _)
-                            in ApplyOps _ _ i ops2
-                                        (rew [ApplyOps spec2 _ P2]
-                                             (eq_sym (replace_op_proofs_eq _ _))
-                                          in proj2 (spec_iso ops2) model2))).
-
-
-(*** Examples of Isomorphic Interpretations ***)
-
-(* Tactic to prove IsoToSpec instances *)
-Ltac prove_spec_iso :=
-  intro ops;
-  repeat (let t := fresh "t" in
-          let pf := fresh "pf" in
-          destruct ops as [t ops]; destruct ops as [pf ops];
-          try destruct pf);
-  destruct ops; split; compute;
-  [ intro H; destruct H;
-    repeat (first [ assumption | split; [assumption|] | apply I])
-  | intro H; repeat (let Hi := fresh "H" in
-                     destruct H as [Hi H]); constructor; assumption ].
-
-(* Example 1:  op n:nat;  axiom gt1: n > 1 *)
-Class spec_example_1_class (n:nat) : Prop :=
-  { example_1__gt1 : n > 1 }.
-
-(* Isomorphism between spec_example_1 and spec_example_1_class *)
-Instance iso_example_1 : IsoToSpec spec_example_1 spec_example_1_class.
-prove_spec_iso.
-Qed.
-
-(* Example 2:  op n:nat := 2;  (no axioms) *)
-Class spec_example_2_class (n:nat) (n__pf: n = 2) : Prop := { }.
-
-Instance iso_example_2 : IsoToSpec spec_example_2 spec_example_2_class.
-prove_spec_iso.
-Qed.
-
-(* Example 3:  op T:Set := nat;  op n:T__def;  axiom gt1: n > 1 *)
-Class spec_example_3_class (T:Set) (T__pf: T = nat) (n: def T T__pf) : Prop :=
-  { example_3__gt1 : n > 1 }.
-
-Instance iso_example_3 : IsoToSpec spec_example_3 spec_example_3_class.
-prove_spec_iso.
-Qed.
-
-(* Example: lift the spec3 -> spec2 interpretation to an instance function *)
-Instance iso_interp_example_3_2 : forall `{spec_example_2_class}, spec_example_3_class _ _ _ :=
-  toIsoInterp (interp_example_3_2).
-
-(* Example 4: monoids *)
-Class Monoid {T:Set} {m_zero:T} {m_plus:T -> T -> T} : Prop :=
-  {m_zero_left : (forall x, m_plus m_zero x = x);
-   m_zero_right : (forall x, m_plus x m_zero = x);
-   m_plus_assoc : (forall x y z, m_plus x (m_plus y z) = m_plus (m_plus x y) z)}.
-
-Instance iso_example_monoid : IsoToSpec spec_example_monoid (@Monoid).
-prove_spec_iso.
-Qed.
-
-(* Example 4: groups *)
-Class Group {T:Set} {g_zero:T} {g_plus:T -> T -> T} {g_inv:T -> T} : Prop :=
-  {g_zero_left : (forall x, g_plus g_zero x = x);
-   g_zero_right : (forall x, g_plus x g_zero = x);
-   g_plus_assoc : (forall x y z, g_plus x (g_plus y z) = g_plus (g_plus x y) z);
-   g_inv_left : (forall (x:T), g_plus (g_inv x) x = g_zero);
-   g_inv_right : (forall (x:T), g_plus x (g_inv x) = g_zero)}.
-
-Instance iso_example_group : IsoToSpec spec_example_group (@Group).
-prove_spec_iso.
-Qed.
-
-(* Interpretation from Monoid to Group type classes *)
-Program Instance group_as_monoid `{Group} :
-  Monoid (m_zero:=g_zero) (m_plus:=g_plus).
-Next Obligation. apply g_zero_left. Qed.
-Next Obligation. apply g_zero_right. Qed.
-Next Obligation. apply g_plus_assoc. Qed.
+(* FIXME HERE: figure out how to define this! *)
 
 (*
-NOTE: the below loops forever!
-
-Check (@group_as_monoid : IsoInterpretation iso_example_monoid iso_example_group _).
-Check (fromIsoInterp (iso1:=iso_example_monoid)
-                     (iso2:=iso_example_group)
-                     (@group_as_monoid)).
-*)
-
-
-(*** An Alternative Isomorphism to Specs ***)
-
 Class IsoToSpecModels {spec} (ops: spec_ops spec) (P: Prop) : Prop :=
   spec_models_iso : P <-> spec_model spec ops.
 
@@ -1322,6 +568,7 @@ Ltac prove_spec_models_iso :=
     repeat (first [ assumption | split; [assumption|] | apply I])
   | intro H; repeat (let Hi := fresh "H" in
                      destruct H as [Hi H]); constructor; assumption ].
+*)
 
 
 (*** Spec Translations ***)
@@ -1398,23 +645,12 @@ Fixpoint translate_spec xlate spec : Spec :=
                   (fun x x__pf => translate_spec xlate (rest x x__pf))
   end.
 
-(* NOTE: the spec_ops type of a translated spec is in fact equal to that of the
-original spec, but this requires functional extensionality to prove... *)
+(* NOTE: the spec_model type of a translated spec is in fact equal to that of
+the original spec, but this requires functional extensionality to prove... *)
 
-Fixpoint translate_spec_ops xlate spec :
-  spec_ops (translate_spec xlate spec) -> spec_ops spec :=
-  match spec return spec_ops (translate_spec xlate spec) -> spec_ops spec with
-    | Spec_Axioms _ => fun ops => ops
-    | Spec_Cons f T oppred rest =>
-      fun ops =>
-        match ops with
-          | existT _ t_o (existT _ pf_o ops') =>
-            ops_cons t_o pf_o (translate_spec_ops xlate _ ops')
-        end
-  end.
-
-Lemma translate_spec_axioms_impl xlate axioms :
-  conjoin_axioms (translate_spec_axioms xlate axioms) -> conjoin_axioms axioms.
+Lemma interp_translate_spec_axioms xlate axioms :
+  Interpretation (Spec_Axioms axioms)
+                 (Spec_Axioms (translate_spec_axioms xlate axioms)).
   induction axioms.
   intro; assumption.
   destruct axioms; destruct a.
@@ -1424,32 +660,21 @@ Lemma translate_spec_axioms_impl xlate axioms :
   apply IHaxioms; assumption.
 Defined.
 
-(* Build an interpretation from spec to (translate_spec xlate spec) *)
-Program Definition interp_translate_spec xlate spec :
+Fixpoint interp_translate_spec xlate spec :
   Interpretation spec (translate_spec xlate spec) :=
-  mkInterp (translate_spec_ops xlate spec) _.
-Next Obligation.
-revert ops H; induction spec; intros.
-apply (translate_spec_axioms_impl xlate); assumption.
-destruct ops as [t_o ops]; destruct ops as [pf_o ops].
-apply H. assumption.
-Defined.
-
-(* Reverse the translation of spec ops *)
-Fixpoint untranslate_spec_ops xlate spec :
-  spec_ops spec -> spec_ops (translate_spec xlate spec) :=
-  match spec return spec_ops spec -> spec_ops (translate_spec xlate spec) with
-    | Spec_Axioms _ => fun ops => ops
+  match spec return Interpretation spec (translate_spec xlate spec) with
+    | Spec_Axioms axioms => interp_translate_spec_axioms xlate axioms
     | Spec_Cons f T oppred rest =>
-      fun ops =>
-        match ops with
-          | existT _ t_o (existT _ pf_o ops') =>
-            ops_cons t_o pf_o (untranslate_spec_ops xlate _ ops')
+      fun model =>
+        match model with
+          | opCons t pf model' =>
+            opCons t pf (interp_translate_spec xlate (rest t pf) model')
         end
   end.
 
-Lemma untranslate_spec_axioms_impl xlate axioms :
-  conjoin_axioms axioms -> conjoin_axioms (translate_spec_axioms xlate axioms).
+Lemma interp_untranslate_spec_axioms xlate axioms :
+  Interpretation (Spec_Axioms (translate_spec_axioms xlate axioms))
+                 (Spec_Axioms axioms).
   induction axioms.
   intro; assumption.
   destruct axioms; destruct a.
@@ -1460,15 +685,17 @@ Lemma untranslate_spec_axioms_impl xlate axioms :
 Defined.
 
 (* Build an interpretation from (translate_spec xlate spec) back to spec *)
-Program Definition interp_untranslate_spec xlate spec :
+Fixpoint interp_untranslate_spec xlate spec :
   Interpretation (translate_spec xlate spec) spec :=
-  mkInterp (untranslate_spec_ops xlate spec) _.
-Next Obligation.
-revert ops H; induction spec; intros.
-apply (untranslate_spec_axioms_impl xlate); assumption.
-destruct ops as [t_o ops]; destruct ops as [pf_o ops].
-apply H. assumption.
-Defined.
+  match spec return Interpretation (translate_spec xlate spec) spec with
+    | Spec_Axioms axioms => interp_untranslate_spec_axioms xlate axioms
+    | Spec_Cons f T oppred rest =>
+      fun model =>
+        match model with
+          | opCons t pf model' =>
+            opCons t pf (interp_untranslate_spec xlate (rest t pf) model')
+        end
+  end.
 
 (* Translate an interpretation *)
 Definition translate_interp {spec1 spec2} xlate
@@ -1491,24 +718,10 @@ Definition interp_cons_strengthen_xlate xlate f1 T (oppred1 oppred2: OpPred T)
                  Interpretation (spec1 t (impl t pf2)) (spec2 t pf2)) :
   Interpretation (Spec_Cons f1 T oppred1 spec1)
                  (Spec_Cons (translate_field xlate f1) T oppred2 spec2) :=
-  mkInterp (fun ops2:spec_ops (Spec_Cons (translate_field xlate f1)
-                                           T oppred2 spec2) =>
-              let (t_o,o) := ops2 in
-              let (pf_o, rest_o) := o in
-              ops_cons t_o (impl _ pf_o) (map_ops (i t_o pf_o) rest_o))
-           (fun ops2 =>
-              match ops2
-                    return spec_model (Spec_Cons (translate_field xlate f1)
-                                                   T oppred2 spec2) ops2 ->
-                           spec_model
-                             (Spec_Cons f1 T oppred1 spec1)
-                             (let (t_o,o) := ops2 in
-                              let (pf_o,rest_o) := o in
-                              ops_cons t_o (impl t_o pf_o) (map_ops (i _ _) rest_o)) with
-                | existT _ t_o (existT _ pf_o rest_o) =>
-                  fun model2 =>
-                    map_model (i t_o pf_o) rest_o model2
-              end).
+  fun model2:spec_model (Spec_Cons (translate_field xlate f1)
+                                   T oppred2 spec2) =>
+    let (t,pf,model2') := model2 in
+    opCons t (impl _ pf) (i t pf model2').
 
 (* Similar to the above, but substitute the definition of an op that is defined
 in the co-domain into the domain spec *)
@@ -1519,24 +732,10 @@ Definition interp_cons_def_xlate xlate f1 T (oppred1: OpPred T) t2
                  Interpretation (spec1 t2 oppred1_pf) (spec2 t pf2)) :
   Interpretation (Spec_Cons f1 T oppred1 spec1)
                  (Spec_Cons (translate_field xlate f1) T (Pred_Eq t2) spec2) :=
-  mkInterp (fun ops2:spec_ops (Spec_Cons (translate_field xlate f1)
-                                           T (Pred_Eq t2) spec2) =>
-              let (t_o,o) := ops2 in
-              let (pf_o, rest_o) := o in
-              ops_cons t2 oppred1_pf (map_ops (i t_o pf_o) rest_o))
-           (fun ops2 =>
-              match ops2
-                    return spec_model (Spec_Cons (translate_field xlate f1)
-                                                   T (Pred_Eq t2) spec2) ops2 ->
-                           spec_model
-                             (Spec_Cons f1 T oppred1 spec1)
-                             (let (t_o,o) := ops2 in
-                              let (pf_o,rest_o) := o in
-                              ops_cons t2 oppred1_pf (map_ops (i _ _) rest_o)) with
-                | existT _ t_o (existT _ pf_o rest_o) =>
-                  fun model2 =>
-                    map_model (i t_o pf_o) rest_o model2
-              end).
+  fun model2:spec_model (Spec_Cons (translate_field xlate f1)
+                                T (Pred_Eq t2) spec2) =>
+     let (t,pf,model2') := model2 in
+     opCons t2 oppred1_pf (i t pf model2').
 
 (* Similar to the above, but allow the field types to be provably, not just
 definitionally, equal *)
@@ -1548,24 +747,10 @@ Definition interp_cons_strengthen_xlate_eq xlate f1 T1 T2 (oppred1: OpPred T1)
                  Interpretation (spec1 (rew eT in t) (impl t pf2)) (spec2 t pf2)) :
   Interpretation (Spec_Cons f1 T1 oppred1 spec1)
                  (Spec_Cons (translate_field xlate f1) T2 oppred2 spec2) :=
-  mkInterp (fun ops2:spec_ops (Spec_Cons (translate_field xlate f1)
-                                           T2 oppred2 spec2) =>
-              let (t_o,o) := ops2 in
-              let (pf_o, rest_o) := o in
-              ops_cons (rew eT in t_o) (impl _ pf_o) (map_ops (i t_o pf_o) rest_o))
-           (fun ops2 =>
-              match ops2
-                    return spec_model (Spec_Cons (translate_field xlate f1)
-                                                   T2 oppred2 spec2) ops2 ->
-                           spec_model
-                             (Spec_Cons f1 T1 oppred1 spec1)
-                             (let (t_o,o) := ops2 in
-                              let (pf_o,rest_o) := o in
-                              ops_cons (rew eT in t_o) (impl t_o pf_o) (map_ops (i _ _) rest_o)) with
-                | existT _ t_o (existT _ pf_o rest_o) =>
-                  fun model2 =>
-                    map_model (i t_o pf_o) rest_o model2
-              end).
+  fun model2:spec_model (Spec_Cons (translate_field xlate f1)
+                                   T2 oppred2 spec2) =>
+    let (t,pf,model2') := model2 in
+    opCons (rew eT in t) (impl _ pf) (i t pf model2').
 
 (* Tactic to prove a "simple" interpretation, which is one where none of the ops
 have to be re-ordered, but where the fields can be translated between the domain
@@ -1583,6 +768,7 @@ Ltac intros_for_cons_op f oppred :=
      | _ => idtac
    end) *)
   idtac.
+(*
 Ltac prove_simple_interp xlate :=
   let next :=
       lazymatch goal with
@@ -1627,6 +813,7 @@ Ltac prove_simple_interp xlate :=
     in
       next
 .
+*)
 
 (* Old version *)
 (*
@@ -1656,9 +843,6 @@ Ltac interp_tactic :=
 
 
 (*** Refinement ***)
-
-(* Helper wrapper around the refine tactic *)
-Ltac specware_refine arg := refine arg.
 
 (* A refinement import into spec is some spec', an interpretation from spec' to
 spec, and a type that is isomorphic to spec' *)
@@ -1739,6 +923,7 @@ Definition refinement_compose {spec}
   end.
 
 (* Apply a spec substitution to a refinement *)
+(*
 Definition refinement_subst_noimport {spec spec1 spec2}
            (R: RefinementOf spec) (overlap: SpecOverlap (ref_spec _ R) spec1)
            (i: Interpretation spec1 spec2) : RefinementOf spec :=
@@ -1787,6 +972,7 @@ Definition refinement_subst_xlate {spec spec1 spec2}
                                     imp (spec_subst_interp1
                                            overlap (translate_interp xlate i))) imps) |}
   end.
+*)
 
 (* Translate a refinement *)
 Definition refinement_translate {spec}
